assume is replaced with a lemma to bring in valid transition to abstraction function

share/pulse/examples/dice/dpe/SPDM7.fst
@@ -249,6 +249,31 @@ let hash_result_success_no_sign (tr0:trace{has_full_state_info (current_state tr
                   b_resp 
                   (current_transcript tr1))
 
+let valid_transition_lemma
+  (tr0:trace{has_full_state_info (current_state tr0)})
+  (rep:repr)
+  (rep_new:repr{~(all_zeros_hash_transcript rep_new.transcript)})
+  : Lemma
+    (requires  (G_Initialized? (current_state tr0) \/ G_Recv_no_sign_resp? (current_state tr0)) /\
+               (G_Initialized? (current_state tr0) ==>
+                          (all_zeros_hash_transcript rep.transcript) /\
+                          (G_Initialized rep == current_state tr0) /\
+                          (rep.signing_pub_key_repr == rep_new.signing_pub_key_repr /\
+                           rep.key_size_repr = rep_new.key_size_repr )) /\
+                
+               (G_Recv_no_sign_resp? (current_state tr0) ==>
+                          ~(all_zeros_hash_transcript rep.transcript) /\
+                          (G_Recv_no_sign_resp rep == current_state tr0) /\
+                          (rep.signing_pub_key_repr == rep_new.signing_pub_key_repr /\
+                           rep.key_size_repr = rep_new.key_size_repr /\
+                          (exists req_size req resp_size resp hash_algo. 
+                             hash_of hash_algo rep.transcript req_size req resp_size resp rep_new.transcript)))
+    )
+    (ensures valid_transition tr0 (G_Recv_no_sign_resp rep_new)) =
+    match (current_state tr0) with
+    | G_Initialized rep -> ()
+    | G_Recv_no_sign_resp rep -> ()
+
 
 fn
 no_sign_resp_aux
@@ -275,6 +300,12 @@ no_sign_resp_aux
                 (rep.signing_pub_key_repr == (current_key tr0)) /\
                 (rep.key_size_repr == (current_key_size tr0)) /\
                 (G_Recv_no_sign_resp? (current_state tr0) \/ G_Initialized? (current_state tr0)) /\
+                (G_Initialized? (current_state tr0) ==>
+                          (all_zeros_hash_transcript rep.transcript) /\
+                          (G_Initialized rep == current_state tr0)) /\
+                (G_Recv_no_sign_resp? (current_state tr0) ==>
+                          ~(all_zeros_hash_transcript rep.transcript) /\
+                          (G_Recv_no_sign_resp rep == current_state tr0)) /\
                 res.status == Success) **
            C.ghost_pcm_pts_to 
                   (get_state_data c).g_trace_ref
@@ -321,15 +352,33 @@ no_sign_resp_aux
      assert_ (V.pts_to curr_state_transcript new_g_transcript');
      hash hash_algo curr_state_transcript ctx.resp_size ctx.resp #new_g_transcript' #b_resp #p_resp;
      assert_ (V.pts_to curr_state_transcript new_g_transcript);
+     assert_ (pure (Seq.equal new_g_transcript' (hash_seq hash_algo curr_g_transcript req_size b_req)));
+     assert_ (pure (Seq.equal new_g_transcript (hash_seq hash_algo new_g_transcript' ctx.resp_size b_resp)));
+
+     assert_ (pure (Seq.equal new_g_transcript (hash_seq hash_algo (hash_seq hash_algo curr_g_transcript req_size b_req) 
+                                                    ctx.resp_size b_resp)));
+     assert_ (pure (hash_of hash_algo curr_g_transcript req_size b_req ctx.resp_size b_resp new_g_transcript));
+
+     assert_ (pure (rep.transcript == curr_g_transcript));
      
      //create a new state data record with the new transcript
     //creation of the ghost session data storage
     let rep_new = {key_size_repr = curr_g_key_size; signing_pub_key_repr = curr_g_key; transcript = new_g_transcript};
-         
+    assert_ (pure (~(all_zeros_hash_transcript rep_new.transcript))); 
+    assert_ (pure (rep_new.transcript == new_g_transcript));
+    assert_ (pure ((rep.signing_pub_key_repr == rep_new.signing_pub_key_repr /\
+                    rep.key_size_repr = rep_new.key_size_repr )));
+    
+    
+    assert_ (pure (hash_of hash_algo rep.transcript req_size b_req ctx.resp_size b_resp rep_new.transcript));
+
+    assert_ (pure (exists req_size req resp_size resp hash_algo. 
+                             hash_of hash_algo rep.transcript req_size req resp_size resp rep_new.transcript));
     //Trace ref creation-----------------------------------------------------------------------------------------------------------
     //new trace----------------------------------------------------------------------------------------------------------------
     //bring in a lemma to prove this
-    assume_ (pure(valid_transition tr0 (G_Recv_no_sign_resp rep_new)));
+    valid_transition_lemma tr0 rep rep_new;
+    assert_ (pure(valid_transition tr0 (G_Recv_no_sign_resp rep_new)));
 
     let tr1 = next_trace tr0 (G_Recv_no_sign_resp rep_new);
 
@@ -398,7 +447,6 @@ no_sign_resp_aux
         
      fin
 }
-
 
 fn no_sign_resp1
   (ctx:parser_context)
@@ -488,7 +536,7 @@ fn no_sign_resp1
           
           rewrite (C.ghost_pcm_pts_to (get_state_data (Initialized st)).g_trace_ref (Some #perm 1.0R, tr0)) as
                    (C.ghost_pcm_pts_to (get_state_data c).g_trace_ref (Some #perm 1.0R, tr0));
-
+          
           let ret = no_sign_resp_aux ctx req_size req c st rep res #tr0 #b_resp #b_req #p_req #p_resp;
           
           assert_ (pure(current_state tr0 == G_Initialized rep));
